theories/Equiv/SimI.v
@@ -27,7 +27,7 @@ Definition irel := rel3 simtype (fun _ : simtype => I.state)
 
 Coercion labN : lab >-> nat.
 
-Definition paramrel A (PR:ProofRelationI A) AL L L' :=
+Definition paramrel A (PR:ProofRelationI A)  AL L L' :=
   forall (f f':lab) Z s i Z' s' i' a,
     IndexRelI AL f f'
     -> get AL f a
